template-coq/theories/Universes.v
@@ -18,8 +18,6 @@ Class Evaluable (A : Type) := val : valuation -> A -> Z.
 
 Module Level.
   Inductive t_ : Set :=
-  | lProp
-  | lSProp
   | lSet
   | Level (_ : string)
   | Var (_ : nat) (* these are debruijn indices *).
@@ -28,13 +26,7 @@ Module Level.
 
   Definition is_small (x : t) :=
     match x with
-    | lSProp | lProp | lSet => true
-    | _ => false
-    end.
-
-  Definition is_prop (x : t) :=
-    match x with
-    | lProp => true
+    | lSet => true
     | _ => false
     end.
 
@@ -52,8 +44,6 @@ Module Level.
 
   Global Instance Evaluable : Evaluable t
     := fun v l => match l with
-               | lSProp => -2 (* CHECKME:SPROP: Not sure if it's a valid value *)
-               | lProp => -1
                | lSet => 0
                | Level s => Z.pos (v.(valuation_mono) s)
                | Var x => Z.of_nat (v.(valuation_poly) x)
@@ -63,12 +53,6 @@ Module Level.
   (* CHECKME:SPROP: [SProp] is added in the same way as [Prop], seems to match [univ.ml] *)
   Definition compare (l1 l2 : t) : comparison :=
     match l1, l2 with
-    | lSProp, lSProp => Eq
-    | lSProp, _ => Lt
-    | _, lSProp => Gt
-    | lProp, lProp => Eq
-    | lProp, _ => Lt
-    | _, lProp => Gt
     | lSet, lSet => Eq
     | lSet, _ => Lt
     | _, lSet => Gt
@@ -87,13 +71,6 @@ Module Level.
   Defined.
 
   Inductive lt_ : t -> t -> Prop :=
-  | ltSPropProp : lt_ lSProp lProp
-  | ltSPropSet : lt_ lSProp lSet
-  | ltSPropLevel s : lt_ lSProp (Level s)
-  | ltSPropVar n : lt_ lSProp (Var n)
-  | ltPropSet : lt_ lProp lSet
-  | ltPropLevel s : lt_ lProp (Level s)
-  | ltPropVar n : lt_ lProp (Var n)
   | ltSetLevel s : lt_ lSet (Level s)
   | ltSetVar n : lt_ lSet (Var n)
   | ltLevelLevel s s' : string_lt s s' -> lt_ (Level s) (Level s')
@@ -105,10 +82,10 @@ Module Level.
   Definition lt_strorder : StrictOrder lt.
   Proof.
     constructor.
-    - intros [| | | | ] X; inversion X.
+    - intros [| |] X; inversion X.
       eapply string_lt_irreflexive; tea.
       eapply Nat.lt_irrefl; tea.
-    - intros [| | | |] [| | | |] [| | | |] X1 X2;
+    - intros [| |] [| |] [| |] X1 X2;
         inversion X1; inversion X2; constructor.
       eapply transitive_string_lt; tea.
       etransitivity; tea.
@@ -258,14 +235,11 @@ Module NoPropLevel.
 
   Definition eq_leibniz (x y : t) : eq x y -> x = y := id.
 
-  Inductive prop_level := plProp | plSProp.
-  Definition of_level (l : Level.t) : t + prop_level :=
+  Definition of_level (l : Level.t) : t :=
     match l with
-    | Level.lSProp => inr plSProp
-    | Level.lProp => inr plProp
-    | Level.lSet => inl lSet
-    | Level.Level s => inl (Level s)
-    | Level.Var n => inl (Var n)
+    | Level.lSet => lSet
+    | Level.Level s => Level s
+    | Level.Var n => Var n
     end.
 
   Definition to_level (l : t) : Level.t :=
@@ -276,7 +250,7 @@ Module NoPropLevel.
     end.
 
   Lemma of_to_level l
-    : of_level (to_level l) = inl l.
+    : of_level (to_level l) = l.
   Proof.
     destruct l; reflexivity.
   Qed.
@@ -304,80 +278,50 @@ Coercion NoPropLevel.to_level : NoPropLevel.t >-> Level.t.
 
 Module UnivExpr.
   (* npe = no prop expression, +1 if true *)
-  Inductive t_ := lProp | lSProp | npe (e : NoPropLevel.t * bool).
+  Inductive t_ := npe (e : NoPropLevel.t * bool).
 
   Definition t := t_.
 
   Global Instance Evaluable : Evaluable t
     := fun v l => match l with
-               | lSProp => -2
-               | lProp => -1
                | npe (l, b) => (if b then 1 else 0) + val v l
                end.
 
 
+  Definition get_level (e : t) : Level.t :=
+    match e with
+    | npe (l, _) => l
+    end.
+
+  Definition get_noprop (e : UnivExpr.t) :=
+    match e with
+    | npe (l, _) => Some l
+    end.
+
   Definition is_small (e : t) : bool :=
     match e with
-    | lProp
     | npe (NoPropLevel.lSet, false) => true
     | _  => false
     end.
 
   Definition is_level (e : t) : bool :=
     match e with
-    | lProp
     | npe (_, false) => true
     | _  => false
     end.
 
-  Definition is_prop (e : t) : bool :=
-    match e with
-    | lProp => true
-    | _  => false
-    end.
-
-  Definition is_sprop (e : t) : bool :=
-    match e with
-    | lSProp => true
-    | _  => false
-    end.
-
-  Definition get_level (e : t) : Level.t :=
-    match e with
-    | lSProp => Level.lSProp
-    | lProp => Level.lProp
-    | npe (l, _) => l
-    end.
-
-  Definition get_noprop (e : UnivExpr.t) :=
-    match e with
-    | lSProp => None
-    | lProp => None
-    | npe (l, _) => Some l
-    end.
-
   Definition make (l : Level.t) : t :=
-    match NoPropLevel.of_level l with
-    | inr NoPropLevel.plProp => lProp
-    | inr NoPropLevel.plSProp => lSProp
-    | inl l => npe (l, false)
-    end.
+    npe (NoPropLevel.of_level l, false).
 
-  Definition prop : t := lProp.
   Definition set : t := npe (NoPropLevel.lSet, false).
   Definition type1 : t := npe (NoPropLevel.lSet, true).
 
   (* Used for (un)quoting. *)
   Definition from_kernel_repr (e : Level.t * bool) : t
-    := match NoPropLevel.of_level e.1 with
-       | inl l => npe (l, e.2)
-       | inr NoPropLevel.plSProp => lSProp
-       | inr NoPropLevel.plProp => lProp
-       end.
+    := npe (NoPropLevel.of_level e.1, e.2).
+
   Definition to_kernel_repr (e : t) : Level.t * bool
     := match e with
-       | lProp => (Level.lProp, false)
-       | lSProp => (Level.lSProp, false)
        | npe (l, b) => (NoPropLevel.to_level l, b)
        end.
 
@@ -386,9 +330,6 @@ Module UnivExpr.
   Definition eq_equiv : Equivalence eq := _.
 
   Inductive lt_ : t -> t -> Prop :=
-  | ltUnivExpr000 : lt_ lSProp lProp   (* CHECKME:SPROP: not sure if it's right*)
-  | ltUnivExpr00 e : lt_ lSProp (npe e)
-  | ltUnivExpr0 e : lt_ lProp (npe e)
   | ltUnivExpr1 l : lt_ (npe (l, false)) (npe (l, true))
   | ltUnivExpr2 l l' b b' : NoPropLevel.lt l l' -> lt_ (npe (l, b)) (npe (l', b')).
 
@@ -409,12 +350,6 @@ Module UnivExpr.
 
   Definition compare (x y : t) : comparison :=
     match x, y with
-    | lSProp, lSProp => Eq
-    | lSProp, _ => Lt
-    | _, lSProp => Gt
-    | lProp, lProp => Eq
-    | lProp, _ => Lt
-    | _, lProp => Gt
     | npe (l1, b1), npe (l2, b2) =>
       match NoPropLevel.compare l1 l2 with
       | Eq => bool_compare b1 b2
@@ -425,7 +360,7 @@ Module UnivExpr.
   Definition compare_spec :
     forall x y : t, CompareSpec (x = y) (lt x y) (lt y x) (compare x y).
   Proof.
-    intros [| | []] [| | []]; cbn; repeat constructor.
+    intros [[]] [[]]; cbn; repeat constructor.
     destruct (NoPropLevel.compare_spec t0 t1); repeat constructor; tas.
     subst. destruct b, b0; repeat constructor.
   Qed.
@@ -450,42 +385,16 @@ Module UnivExpr.
     destruct l; cbnr.
   Qed.
 
-  Lemma val_minus_two e v : -2 <= val v e.
+  Lemma val_zero e v : 0 <= val v e.
   Proof.
-    destruct e as [| | [[] b]]; cbn; try destruct b; try lia.
+    destruct e as [[[] b]]; cbn; try destruct b; try lia.
   Qed.
 
-  Lemma is_prop_val e : is_prop e -> forall v, val v e = -1.
-  Proof.
-    destruct e as [| | [[] []]]; cbn; try reflexivity; try discriminate.
-  Qed.
+  (* Lemma val_minus_one e v : -1 <= val v e. *)
+  (* Proof. *)
+  (*   destruct e as [[[] b]]; cbn; try destruct b; try lia. *)
+  (* Qed. *)
 
-  Lemma val_is_sprop e v : val v e <= -2 ->is_sprop e.
-  Proof.
-    destruct e as [| | [[] b]] eqn:H; cbnr; try destruct b; auto; lia.
-  Qed.
-
-  Lemma val_is_prop_or_sprop e v : val v e <= -1 -> is_prop e \/ is_sprop e.
-  Proof.
-    destruct e as [| | [[] b]] eqn:H; cbnr; try destruct b; auto; lia.
-  Qed.
-
-  Lemma is_prop_val_false e :
-    is_prop e = false /\ is_sprop e = false -> forall v, 0 <= val v e.
-  Proof.
-    intros [He1 He2] v.
-    pose proof (val_is_prop_or_sprop e v).
-    pose proof (val_minus_two e v).
-    destruct (Z_le_gt_dec (val v e) (-1));[| lia].
-    forward H; tas. rewrite He1 in H. rewrite He2 in H. intuition;discriminate.
-  Qed.
-
-  Lemma val_is_prop_false e v :
-    0 <= val v e -> is_prop e = false.
-  Proof.
-    pose proof (is_prop_val e) as H. destruct (is_prop e); cbnr.
-    rewrite (H eq_refl v). lia.
-  Qed.
 End UnivExpr.
 
 Module UnivExprSet := MSetList.MakeWithLeibniz UnivExpr.
@@ -498,20 +407,31 @@ Module Universe.
         - sorted
         - without duplicate
         - non empty *)
-  Record t := { t_set : UnivExprSet.t ;
-                t_ne  : UnivExprSet.is_empty t_set = false }.
+  Record t0 := { t_set : UnivExprSet.t ;
+                 t_ne  : UnivExprSet.is_empty t_set = false }.
 
-  Coercion t_set : t >-> UnivExprSet.t.
+  Inductive t_ :=
+    lProp | lSProp | lnpe (_ : t0).
+
+  Definition t := t_.
+
+  Coercion t_set : t0 >-> UnivExprSet.t.
 
   Definition eqb (u1 u2 : t) : bool :=
-    UnivExprSet.equal u1.(t_set) u2.(t_set).
+    match u1, u2 with
+    | lSProp, lSProp => true
+    | lProp, lProp => true
+    | lnpe e1, lnpe e2 => UnivExprSet.equal e1.(t_set) e2.(t_set)
+    | _,_ => false
+    end.
 
-  Definition make' (e : UnivExpr.t) : t
+  Definition make' (e : UnivExpr.t) : t0
     := {| t_set := UnivExprSet.singleton e;
           t_ne := eq_refl |}.
 
   (** Create a universe representing the given level. *)
-  Definition make (l : Level.t) : t := make' (UnivExpr.make l).
+  Definition make (l : Level.t) : t :=
+    lnpe (make' (UnivExpr.make l)).
 
   Lemma not_Empty_is_empty s :
     ~ UnivExprSet.Empty s -> UnivExprSet.is_empty s = false.
@@ -520,7 +440,7 @@ Module Universe.
     apply H. now apply UnivExprSetFact.is_empty_2 in H'.
   Qed.
 
-  Program Definition add (e : UnivExpr.t) (u : t) : t
+  Program Definition add (e : UnivExpr.t) (u : t0) : t0
     := {| t_set := UnivExprSet.add e u |}.
   Next Obligation.
     apply not_Empty_is_empty; intro H.
@@ -528,13 +448,19 @@ Module Universe.
     left; reflexivity.
   Qed.
 
+  Definition add_to_exprs (e : UnivExpr.t) (u : t) : t :=
+    match u with
+    | lSProp |lProp => u
+    | lnpe l => lnpe (add e l)
+    end.
+
   Lemma add_spec e u e' :
     UnivExprSet.In e' (add e u) <-> e' = e \/ UnivExprSet.In e' u.
   Proof.
     apply UnivExprSet.add_spec.
   Qed.
 
-  Definition add_list : list UnivExpr.t -> t -> t
+  Definition add_list : list UnivExpr.t -> t0 -> t0
     := List.fold_left (fun u e => add e u).
 
   Lemma add_list_spec l u e :
@@ -557,45 +483,72 @@ Module Universe.
         * apply add_spec; right. apply IHl0. now right.
   Qed.
 
+  Definition add_list_to_exprs (es : list UnivExpr.t) (u : t) : t :=
+    match u with
+    | lSProp |lProp => u
+    | lnpe l => lnpe (add_list es l)
+    end.
+
   (** Test if the universe is a lub of levels or contains +n's. *)
-  Definition is_levels : t -> bool
-    := UnivExprSet.for_all UnivExpr.is_level.
+  Definition is_levels (u : t) : bool :=
+      match u with
+      | lProp | lSProp => true
+      | lnpe l =>  UnivExprSet.for_all UnivExpr.is_level l
+      end.
 
   (** Test if the universe is a level or an algebraic universe. *)
   Definition is_level (u : t) : bool :=
-    (UnivExprSet.cardinal u =? 1)%nat &&  is_levels u.
+    match u with
+    | lProp | lSProp => true
+    | lnpe l => (UnivExprSet.cardinal l =? 1)%nat && is_levels u
+    end.
 
-  Definition is_small  : t -> bool :=
-    UnivExprSet.for_all UnivExpr.is_small.
+  Definition is_small (u : t) : bool :=
+    match u with
+      | lProp | lSProp => true
+      | lnpe l => UnivExprSet.for_all UnivExpr.is_small l
+    end.
 
-  Definition is_sprop  : t -> bool :=
-    UnivExprSet.for_all UnivExpr.is_sprop.
+  Definition is_sprop (u : t) : bool :=
+    match u with
+      | lSProp => true
+      | _ => false
+    end.
 
-  Definition is_prop  : t -> bool :=
-    UnivExprSet.for_all UnivExpr.is_prop.
+  Definition is_prop (u : t) : bool :=
+    match u with
+      | lProp => true
+      | _ => false
+    end.
 
-  Definition type0m : t := make Level.lProp.
   Definition type0 : t := make Level.lSet.
-  Definition type1 : t := make' UnivExpr.type1.
+  Definition type1 : t := lnpe (make' UnivExpr.type1).
 
-  (* Used for (un)quoting. *)
+  (* Used for quoting. *)
   Definition from_kernel_repr (e : Level.t * bool) (es : list (Level.t * bool)) : t
-    := add_list (map UnivExpr.from_kernel_repr es)
-                (make' (UnivExpr.from_kernel_repr e)).
-  Definition to_kernel_repr (u : t) : list (Level.t * bool)
-    := map (UnivExpr.to_kernel_repr) (UnivExprSet.elements u).
+    := lnpe (add_list (map UnivExpr.from_kernel_repr es)
+                (make' (UnivExpr.from_kernel_repr e))).
+
+  (* Definition uex_to_kernel_repr (e : UnivExpr.t) : Level.t * bool := *)
+  (*   match e with *)
+  (*   | UnivExpr.npe (l, b) => (NoPropLevel.to_level l, b) *)
+  (*   end. *)
+
+  (* Definition to_kernel_repr (u : t) : list (Level.t * bool) *)
+  (*   :=  map (UnivExpr.to_kernel_repr) (UnivExprSet.elements u). *)
+  (* match u with *)
+  (*      | lProp => [(Level.lProp, false)] *)
+  (*      | lSProp => [(Level.lSProp, false)] *)
+  (*      | lnpe l => map uex_to_kernel_repr (UnivExprSet.elements l) *)
+  (*      end. *)
 
   (** The universe strictly above FOR TYPING (not cumulativity) *)
   Definition super (l : Level.t) : t :=
-    match NoPropLevel.of_level l with
-    | inr _ => type1
-    | inl NoPropLevel.lSet => type1
-    | inl l => make' (UnivExpr.npe (l, true))
-    end.
+    lnpe (make' (UnivExpr.npe (NoPropLevel.of_level l, true))).
 
   (** The non empty / sorted / without dup list of univ expressions, the
       components of the pair are the head and the tail of the (non empty) list *)
-  Program Definition exprs (u : t) : UnivExpr.t * list UnivExpr.t
+  Program Definition exprs (u : t0) : UnivExpr.t * list UnivExpr.t
     := match UnivExprSet.elements u with
        | [] => False_rect _ _
        | e :: l => (e, l)
@@ -611,8 +564,8 @@ Module Universe.
   Lemma exprs_make' e : Universe.exprs (Universe.make' e) = (e, []).
   Proof. reflexivity. Defined.
 
-  Lemma exprs_make l : Universe.exprs (Universe.make l) = (UnivExpr.make l, []).
-  Proof. reflexivity. Defined.
+  (* Lemma exprs_make l : Universe.exprs (Universe.make l) = (UnivExpr.make l, []). *)
+  (* Proof. reflexivity. Defined. *)
 
 
   Lemma exprs_spec u :
@@ -646,7 +599,7 @@ Module Universe.
     now destruct (Universe.exprs u).
   Qed.
 
-  Lemma In_exprs (u : t) (e : UnivExpr.t) :
+  Lemma In_exprs (u : t0) (e : UnivExpr.t) :
     UnivExprSet.In e u
     <-> e = (Universe.exprs u).1 \/ In e (Universe.exprs u).2.
   Proof.
@@ -657,7 +610,7 @@ Module Universe.
     eapply or_iff_compat_l. apply InA_In_eq.
   Qed.
 
-  Lemma In_exprs_rev (u : t) (e : UnivExpr.t) :
+  Lemma In_exprs_rev (u : t0) (e : UnivExpr.t) :
     UnivExprSet.In e u
     <-> e = (Universe.exprs u).1 \/ In e (List.rev (Universe.exprs u).2).
   Proof.
@@ -665,7 +618,7 @@ Module Universe.
     apply or_iff_compat_l. apply in_rev.
   Qed.
 
-  Definition map (f : UnivExpr.t -> UnivExpr.t) (u : t) : t :=
+  Definition map (f : UnivExpr.t -> UnivExpr.t) (u : t0) : t0 :=
     let '(e, l) := exprs u in
     add_list (List.map f l) (make' (f e)).
 
@@ -689,13 +642,11 @@ Module Universe.
 
   Definition try_suc
     := map (fun l => match l with
-                  | UnivExpr.lSProp => UnivExpr.type1
-                  | UnivExpr.lProp => UnivExpr.type1
                   | UnivExpr.npe (l, _) => UnivExpr.npe (l, true)
                   end).
 
-  (** The l.u.b. of 2 universes *)
-  Program Definition sup (u v : t) : t :=
+    (** The l.u.b. of 2 non-prop universes *)
+  Program Definition sup (u v : t0) : t0 :=
     {| t_set := UnivExprSet.union u v |}.
   Next Obligation.
     apply not_Empty_is_empty; intro H.
@@ -706,18 +657,31 @@ Module Universe.
     rewrite t_ne in HH; discriminate.
   Qed.
 
+  Definition universe_sup (u v : t) : t :=
+    match u,v with
+    | lSProp, lProp => lProp
+    | lProp, lSProp => lProp
+    | (lSProp | lProp), u' => u'
+    | u', (lSProp | lProp) => u'
+    | lnpe l1, lnpe l2  => lnpe (sup l1 l2)
+    end.
+
+  Definition get_univ_exprs (u : t) (H1 : is_prop u = false) (H2 : is_sprop u = false) : t0.
+  destruct u; try discriminate;easy. Defined.
+
   (** Type of a product *)
   Definition sort_of_product (domsort rangsort : t) :=
-    (* Prop impredicativity *)
-    if Universe.is_prop rangsort then rangsort
-    else Universe.sup domsort rangsort.
+    (* Prop and SProp impredicativity *)
+    if Universe.is_prop rangsort || Universe.is_sprop rangsort then rangsort
+    else Universe.universe_sup domsort rangsort.
 
   Lemma eqb_refl u : eqb u u.
   Proof.
-    apply UnivExprSet.equal_spec. reflexivity.
+    destruct u;auto.
+    now apply UnivExprSet.equal_spec.
   Qed.
 
-  Lemma elements_not_empty (u : Universe.t) : UnivExprSet.elements u <> [].
+  Lemma elements_not_empty (u : Universe.t0) : UnivExprSet.elements u <> [].
   Proof.
     destruct u as [u1 u2]; cbn; intro e.
     unfold UnivExprSet.is_empty, UnivExprSet.elements,
@@ -726,15 +690,24 @@ Module Universe.
   Qed.
 
   Definition get_is_level (u : t) : option Level.t :=
-    match UnivExprSet.elements u with
-    | [UnivExpr.lProp] => Some Level.lProp
-    | [UnivExpr.npe (l, false)] => Some (NoPropLevel.to_level l)
-    | _ => None
+    match u with
+    | lSProp => None
+    | lProp => None
+    | lnpe l => match UnivExprSet.elements l with
+                 [UnivExpr.npe (l, false)] => Some (NoPropLevel.to_level l)
+               | _ => None
+               end
     end.
 
-  Global Instance Evaluable : Evaluable t
+  Global Instance Evaluable' : Evaluable t0
     := fun v u => let '(e, u) := Universe.exprs u in
                List.fold_left (fun n e => Z.max (val v e) n) u (val v e).
+
+  Global Instance Evaluable : Evaluable t
+    := fun v u => match u with
+            | lSProp | lProp => -1
+            | lnpe l => val v l
+            end.
 
   Lemma val_make' v e
     : val v (make' e) = val v e.
@@ -759,10 +732,11 @@ Module Universe.
   Proof.
     destruct x, y; try now inversion 1.
   Qed.
+
 End Universe.
 
 (** This coercion allows to see the universes as a [UnivExprSet.t] *)
-Coercion Universe.t_set : Universe.t >-> UnivExprSet.t.
+Coercion Universe.t_set : Universe.t0 >-> UnivExprSet.t.
 
 
 Ltac u :=
@@ -771,16 +745,16 @@ Ltac u :=
  (* change ConstraintSet.elt with UnivConstraint.t in *. *)
 
 
-Lemma val_fold_right (u : Universe.t) v :
+Lemma val_fold_right (u : Universe.t0) v :
   val v u = fold_right (fun e x => Z.max (val v e) x) (val v (Universe.exprs u).1)
                        (List.rev (Universe.exprs u).2).
 Proof.
-  unfold val at 1, Universe.Evaluable.
+  unfold val at 1, Universe.Evaluable,Universe.Evaluable'.
   destruct (Universe.exprs u).
   now rewrite fold_left_rev_right.
 Qed.
 
-Lemma val_In_le (u : Universe.t) v e :
+Lemma val_In_le (u : Universe.t0) v e :
   UnivExprSet.In e u -> val v e <= val v u.
 Proof.
   intro H. rewrite val_fold_right.
@@ -792,7 +766,7 @@ Proof.
     + specialize (IHl0 H0). lia.
 Qed.
 
-Lemma val_In_max (u : Universe.t) v :
+Lemma val_In_max (u : Universe.t0) v :
   exists e, UnivExprSet.In e u /\ val v e = val v u.
 Proof.
   eapply iff_ex. {
@@ -809,7 +783,7 @@ Proof.
       destruct H1 as [H1|H1]; [now left|right]. now constructor 2.
 Qed.
 
-Lemma val_ge_caract (u : Universe.t) v k :
+Lemma val_ge_caract (u : Universe.t0) v k :
   (forall e, UnivExprSet.In e u -> val v e <= k) <-> val v u <= k.
 Proof.
   split.
@@ -830,7 +804,7 @@ Proof.
   - intros H e He. eapply val_In_le in He. etransitivity; eassumption.
 Qed.
 
-Lemma val_le_caract (u : Universe.t) v k :
+Lemma val_le_caract (u : Universe.t0) v k :
   (exists e, UnivExprSet.In e u /\ k <= val v e) <-> k <= val v u.
 Proof.
   split.
@@ -852,7 +826,8 @@ Proof.
 Qed.
 
 
-Lemma val_caract (u : Universe.t) v k :
+
+Lemma val_caract (u : Universe.t0) v k :
   val v u = k
   <-> (forall e, UnivExprSet.In e u -> val v e <= k)
     /\ exists e, UnivExprSet.In e u /\ val v e = k.
@@ -903,59 +878,79 @@ Proof.
   apply UnivExprSetFact.for_all_b; proper.
 Qed.
 
-Lemma val_minus_one u v :
-  (-2 <= val v u)%Z.
+Lemma val_exprs_zero v (l : Universe.t0) :
+  (0 <= val v l)%Z.
 Proof.
   rewrite val_fold_right.
-  destruct (Universe.exprs u) as [e u']; clear u; cbn.
+  destruct (Universe.exprs l) as [e u']; clear l; cbn.
   induction (List.rev u'); simpl.
-  - apply UnivExpr.val_minus_two.
-  - pose proof (UnivExpr.val_minus_two a v). lia.
+  - apply UnivExpr.val_zero.
+  - pose proof (UnivExpr.val_zero a v). lia.
+Qed.
+
+Lemma val_minus_one u v :
+  (-1 <= val v u)%Z.
+Proof.
+  destruct u;cbn;try lia.
+  pose proof (val_exprs_zero v t);lia.
+Qed.
+
+Lemma val_universe_sup v u1 u2 :
+  val v (Universe.universe_sup u1 u2) = Z.max (val v u1) (val v u2).
+Proof.
+  assert (Hv : forall l: Universe.t0, 0 <= val v l) by apply val_exprs_zero.
+  destruct u1 as [ | | l1]; destruct u2 as [ | | l2];cbn;try lia.
+  all: try (specialize (Hv l1) as Hv';lia); try (specialize (Hv l2) as Hv';lia).
+  apply val_sup.
 Qed.
 
 Lemma is_prop_val u :
   Universe.is_prop u -> forall v, val v u = -1.
 Proof.
-  unfold Universe.is_prop. rewrite for_all_elements.
-  intros H v. rewrite val_fold_right.
-  rewrite <- (Universe.exprs_spec' u) in H.
-  destruct (Universe.exprs u) as [e l]; simpl in *.
-  apply andb_true_iff in H; destruct H as [He H]; revert H.
-  rewrite <- forallb_rev. induction (List.rev l); simpl.
-  - intros _. apply UnivExpr.is_prop_val; assumption.
-  - intro H; apply andb_true_iff in H; destruct H as [H1 H2].
-    apply UnivExpr.is_prop_val with (v:=v) in H1. now rewrite IHl0, H1.
+  destruct u as [| | u];try discriminate;auto.
 Qed.
+
+Lemma is_sprop_val u :
+  Universe.is_sprop u -> forall v, val v u = -1.
+Proof.
+  destruct u as [| | u];try discriminate;auto.
+Qed.
+
+
+Lemma val_zero_exprs v (l : Universe.t0) : 0 <= val v l.
+Proof.
+  rewrite val_fold_right.
+  destruct (Universe.exprs l) as [e u']; clear l; cbn.
+  induction (List.rev u'); simpl.
+  - destruct e as [npl_expr].
+    destruct npl_expr as [t b].
+    cbn.
+    assert (0 <= val v t) by apply NoPropLevel.val_zero.
+    destruct b;lia.
+  - pose proof (UnivExpr.val_zero a v); lia.
+Qed.
+
 
 Lemma val_is_prop_or_sprop u v :
   val v u <= -1 -> Universe.is_prop u \/ Universe.is_sprop u.
 Proof.
-  unfold Universe.is_prop, Universe.is_sprop. repeat rewrite for_all_elements.
-  rewrite val_fold_right.
-  repeat rewrite <- (Universe.exprs_spec' u).
-  destruct (Universe.exprs u) as [e l]; simpl.
-  replace (forallb UnivExpr.is_prop l) with
-      (forallb UnivExpr.is_prop (List.rev l)) by now rewrite forallb_rev.
-  replace (forallb UnivExpr.is_sprop l) with
-      (forallb UnivExpr.is_sprop (List.rev l)) by now rewrite forallb_rev.
-  induction (List.rev l); cbn.
-  - repeat rewrite andb_true_r. apply UnivExpr.val_is_prop_or_sprop.
-  - intro H. forward IHl0; [lia|].
-    specialize (UnivExpr.val_is_prop_or_sprop a v) as H'. forward H'; [lia|].
-(*     left. apply andb_true_iff. apply andb_true_iff in IHl0. *)
-(*     intuition. *)
-(* Qed. *)
-Admitted.
+  intros H.
+  destruct u;auto;cbn in *.
+  assert (0 <= val v t) by apply val_zero_exprs. lia.
+Qed.
 
-Lemma is_prop_val_false u :
-  Universe.is_prop u = false -> forall v, 0 <= val v u.
+Lemma is_prop_and_is_sprop_val_false u :
+  Universe.is_prop u = false -> Universe.is_sprop u = false -> forall v, 0 <= val v u.
 Proof.
-  intros Hu v.
-  (* pose proof (val_is_prop u v). *)
-  (* pose proof (val_minus_one u v). *)
-  (* destruct (Z_le_gt_dec (val v u) (-1)); [|lia]. *)
-  (* forward H; tas. rewrite Hu in H; discriminate. *)
-Admitted.
+  intros Hp Hsp v.
+  pose proof (val_is_prop_or_sprop u v).
+  pose proof (val_minus_one u v).
+  destruct ( Z_le_gt_dec (val v u) (-1)); [|lia].
+  forward H; tas. unfold is_true in *.
+  destruct H.
+  - rewrite H in Hp; discriminate.
+  - rewrite H in Hsp; discriminate.
+Qed.
 
 Lemma val_is_prop_false u v :
   0 <= val v u -> Universe.is_prop u = false.
@@ -964,21 +959,20 @@ Proof.
   rewrite (H eq_refl v). lia.
 Qed.
 
-
-Lemma eq_univ (u v : Universe.t) :
+Lemma eq_univ (u v : Universe.t0) :
   u = v :> UnivExprSet.t -> u = v.
 Proof.
   destruct u as [u1 u2], v as [v1 v2]; cbn. intros X; destruct X.
   now rewrite (uip_bool _ _ u2 v2).
 Qed.
 
-Lemma eq_univ' (u v : Universe.t) :
+Lemma eq_univ' (u v : Universe.t0) :
   UnivExprSet.Equal u v -> u = v.
 Proof.
   intro H. now apply eq_univ, UnivExprSet.eq_leibniz.
 Qed.
 
-Lemma eq_univ'' (u v : Universe.t) :
+Lemma eq_univ'' (u v : Universe.t0) :
   UnivExprSet.elements u = UnivExprSet.elements v -> u = v.
 Proof.
   intro H. apply eq_univ.
@@ -990,20 +984,29 @@ Qed.
 Lemma get_is_level_correct u l :
   Universe.get_is_level u = Some l -> u = Universe.make l.
 Proof.
-  intro H. apply eq_univ''; cbn. unfold Universe.get_is_level in *.
-  destruct (UnivExprSet.elements u) as [|l0 L]; [discriminate|].
-  destruct l0, L; try discriminate.
-  apply some_inj in H; now subst.
-  destruct e as [? []]; try discriminate.
-  apply some_inj in H; subst. now destruct t.
-  destruct e as [? []]; try discriminate.
+  intro H.
+  destruct u eqn:Hu;cbn in *.
+  - inversion H;subst;reflexivity.
+  - inversion H;subst;reflexivity.
+  - unfold Universe.make.
+    (* apply eq_univ''; cbn. unfold Universe.get_is_level in *. *)
+    destruct (UnivExprSet.elements _) as [|l0 L] eqn:Hu1; [discriminate|].
+    destruct l0, L; try discriminate.
+    * destruct e,b;inversion H;subst.
+      apply f_equal.
+      apply eq_univ'';unfold UnivExpr.make.
+      now rewrite NoPropLevel.of_to_level.
+    * destruct e,b;inversion H;subst.
 Qed.
 
 Lemma eqb_true_iff u v :
   Universe.eqb u v <-> u = v.
 Proof.
   split. 2: intros ->; apply Universe.eqb_refl.
-  intro H. apply eq_univ'. now apply UnivExprSet.equal_spec.
+  intro H.
+  destruct u,v;auto;try discriminate.
+  apply f_equal.
+  apply eq_univ'. now apply UnivExprSet.equal_spec.
 Qed.
 
 Lemma UnivExprSet_for_all_false f u :
@@ -1018,7 +1021,7 @@ Proof.
   right; now rewrite IHl.
 Qed.
 
-Lemma UnivExprSet_For_all_exprs (P : UnivExpr.t -> Prop) (u : Universe.t)
+Lemma UnivExprSet_For_all_exprs (P : UnivExpr.t -> Prop) (u : Universe.t0)
   : UnivExprSet.For_all P u
     <-> P (Universe.exprs u).1 /\ Forall P (Universe.exprs u).2.
 Proof.
@@ -1039,49 +1042,65 @@ Proof.
   intros H. rewrite !UnivExprSet.union_spec. intuition.
 Qed.
 
-Lemma is_prop_sort_sup x1 x2 :
-  Universe.is_prop (Universe.sup x1 x2) -> Universe.is_prop x2.
+Lemma universe_sup_comm x1 x2 :
+  Universe.universe_sup x1 x2 = Universe.universe_sup x2 x1.
 Proof.
-  intro H. apply UnivExprSet.for_all_spec; proper.
-  apply UnivExprSet.for_all_spec in H; proper.
-  intros x HX; apply H.
-  apply UnivExprSet.union_spec; now right.
+  destruct x1,x2;auto.
+  cbn;apply f_equal;apply sup_comm.
 Qed.
+
+Lemma is_prop_sort_sup x1 x2 :
+  Universe.is_prop (Universe.universe_sup x1 x2)
+  -> Universe.is_prop x2 \/ Universe.is_sprop x2 .
+Proof. destruct x1,x2;auto. Qed.
+
+Lemma is_prop_sort_sup' x1 x2 :
+  Universe.is_prop (Universe.universe_sup x1 x2)
+  -> Universe.is_prop x1 \/ Universe.is_sprop x1 .
+Proof. destruct x1,x2;auto. Qed.
+
+Lemma is_prop_or_sprop_sort_sup x1 x2 :
+  Universe.is_sprop (Universe.universe_sup x1 x2) -> Universe.is_sprop x2.
+Proof. destruct x1,x2;auto. Qed.
 
 Lemma is_prop_sort_sup_prop x1 x2 :
   Universe.is_prop x1 && Universe.is_prop x2 ->
-  Universe.is_prop (Universe.sup x1 x2).
-Proof.
-  intro H; apply andP in H as [H1 H2].
-  apply UnivExprSet.for_all_spec; proper.
-  apply UnivExprSet.for_all_spec in H1; proper.
-  apply UnivExprSet.for_all_spec in H2; proper.
-  intros H x.
-  apply UnivExprSet.union_spec in x.
-  destruct x.  now specialize (H1 _ H0).
-  apply (H2 _ H0).
-Qed.
+  Universe.is_prop (Universe.universe_sup x1 x2).
+Proof. destruct x1,x2;auto. Qed.
+
+Lemma is_prop_or_sprop_sort_sup_prop x1 x2 :
+  Universe.is_sprop x1 && Universe.is_sprop x2 ->
+  Universe.is_sprop (Universe.universe_sup x1 x2).
+Proof. destruct x1,x2;auto. Qed.
 
 Lemma is_prop_sup u s :
-  Universe.is_prop (Universe.sup u s)
-  = Universe.is_prop u && Universe.is_prop s.
-Proof.
-  apply iff_is_true_eq_bool; split; intro H.
-  - rewrite (is_prop_sort_sup _ _ H).
-    rewrite sup_comm in H. now rewrite (is_prop_sort_sup _ _ H).
-  - now apply is_prop_sort_sup_prop.
-Qed.
+  Universe.is_prop (Universe.universe_sup u s) ->
+  (Universe.is_prop u \/ Universe.is_sprop u) /\
+  (Universe.is_prop s \/ Universe.is_sprop s).
+Proof. destruct u,s;auto. Qed.
 
+Lemma is_sprop_sup_iff u s :
+  Universe.is_sprop (Universe.universe_sup u s) <->
+  (Universe.is_sprop u /\ Universe.is_sprop s).
+Proof. split;destruct u,s;intuition. Qed.
 
 Lemma is_prop_sort_prod x2 x3 :
-  Universe.is_prop (Universe.sort_of_product x2 x3) -> Universe.is_prop x3.
+  Universe.is_prop (Universe.sort_of_product x2 x3)
+  -> Universe.is_prop x3.
 Proof.
   unfold Universe.sort_of_product.
-  case_eq (Universe.is_prop x3); try reflexivity.
-  intros <-. apply is_prop_sort_sup.
+  destruct x3;cbn;auto.
+  intros;simpl in *;destruct x2;auto.
 Qed.
 
-
+Lemma is_sprop_sort_prod x2 x3 :
+  Universe.is_sprop (Universe.sort_of_product x2 x3)
+  -> Universe.is_sprop x3.
+Proof.
+  unfold Universe.sort_of_product.
+  destruct x3;cbn;auto.
+  intros;simpl in *;destruct x2;auto.
+Qed.
 
 (** Sort families *)
 
@@ -1491,42 +1510,56 @@ Context {cf:checker_flags}.
     intros [H1 H2] v Hv; specialize (H1 v Hv); specialize (H2 v Hv); lled; lia.
   Qed.
 
-
   Lemma leq_universe0_sup_l φ s1 s2 :
-    Universe.is_prop s1 = false -> leq_universe0 φ s1 (Universe.sup s1 s2).
+    Universe.is_prop s1 = false -> Universe.is_sprop s1 = false -> leq_universe0 φ s1 (Universe.universe_sup s1 s2).
   Proof.
-    intros H v Hv. apply is_prop_val_false with (v:=v) in H.
-    rewrite val_sup. unfold lle, llt. destruct prop_sub_type; lia.
+    intros H1 H2 v Hv.
+    specialize (is_prop_and_is_sprop_val_false _ H1 H2 v) as Hzero.
+    rewrite val_universe_sup. unfold lle, llt. destruct prop_sub_type; try lia.
   Qed.
 
   Lemma leq_universe0_sup_r φ s1 s2 :
-    Universe.is_prop s2 = false -> leq_universe0 φ s2 (Universe.sup s1 s2).
+    Universe.is_prop s2 = false -> Universe.is_sprop s2 = false -> leq_universe0 φ s2 (Universe.universe_sup s1 s2).
   Proof.
-    intros H v Hv. apply is_prop_val_false with (v:=v) in H.
-    rewrite val_sup. unfold lle, llt. destruct prop_sub_type; lia.
+    intros H1 H2 v Hv.
+    specialize (is_prop_and_is_sprop_val_false _ H1 H2 v) as Hzero.
+    rewrite val_universe_sup. unfold lle, llt. destruct prop_sub_type; try lia.
   Qed.
 
-  Lemma leq_universe0_sup_l' φ s1 s2 :
-    prop_sub_type -> leq_universe0 φ s1 (Universe.sup s1 s2).
+  Lemma leq_universe0_sup_l' φ (s1 s2 : Universe.t0) :
+    leq_universe0 φ (Universe.lnpe s1) (Universe.lnpe (Universe.sup s1 s2)).
   Proof.
-    intros H v Hv. rewrite val_sup. unfold lle, llt; rewrite H. lia.
+    intros v Hv. cbn. rewrite val_sup. unfold lle, llt.
+    destruct ?.
+    + lia.
+    + specialize (val_zero_exprs v s1) as Hzero.
+      assert (val v s1 < Z.max (val v s1) (val v s2) \/
+              val v s1 = Z.max (val v s1) (val v s2)) by lia.
+      lia.
   Qed.
 
-  Lemma leq_universe0_sup_r' φ s1 s2 :
-    prop_sub_type -> leq_universe0 φ s2 (Universe.sup s1 s2).
+  Lemma leq_universe0_sup_r' φ (s1 s2 : Universe.t0) :
+    leq_universe0 φ (Universe.lnpe s2) (Universe.lnpe (Universe.sup s1 s2)).
   Proof.
-    intros H v Hv. rewrite val_sup. unfold lle, llt; rewrite H. lia.
+    intros v Hv. cbn. rewrite val_sup. unfold lle, llt.
+    destruct ?.
+    + lia.
+    + specialize (val_zero_exprs v s2) as Hzero.
+      assert (val v s2 < Z.max (val v s1) (val v s2) \/
+            val v s2 = Z.max (val v s1) (val v s2)) by lia.
+      lia.
   Qed.
 
-  Lemma leq_universe_product φ s1 s2
+  Lemma leq_universe_product φ (s1 s2 : Universe.t)
     : leq_universe φ s2 (Universe.sort_of_product s1 s2).
   Proof.
     unfold leq_universe; destruct check_univs; [cbn|constructor].
-    unfold Universe.sort_of_product; case_eq (Universe.is_prop s2); intro eq.
-    apply leq_universe0_refl.
-    now apply leq_universe0_sup_r.
+    unfold Universe.sort_of_product.
+    destruct s2; cbn; try apply leq_universe0_refl.
+    destruct s1;cbn;try apply leq_universe0_refl.
+    unfold lle, llt.
+    apply leq_universe0_sup_r'.
   Qed.
-
   (* Rk: [leq_universe φ s1 (sort_of_product s1 s2)] does not hold due to
      impredicativity. *)
 
@@ -1620,7 +1653,7 @@ Class UnivSubst A := subst_instance : Instance.t -> A -> A.
 
 Instance subst_instance_level : UnivSubst Level.t :=
   fun u l => match l with
-          | Level.lSProp | Level.lProp | Level.lSet | Level.Level _ => l
+            Level.lSet | Level.Level _ => l
           | Level.Var n => List.nth n u Level.lSet
           end.
 
@@ -1633,24 +1666,21 @@ Instance subst_instance_cstrs : UnivSubst ConstraintSet.t :=
 
 Instance subst_instance_level_expr : UnivSubst UnivExpr.t :=
   fun u e => match e with
-          | UnivExpr.lSProp => UnivExpr.lSProp
-          | UnivExpr.lProp => UnivExpr.lProp
           | UnivExpr.npe (NoPropLevel.lSet, _)
           | UnivExpr.npe (NoPropLevel.Level _, _) => e
           | UnivExpr.npe (NoPropLevel.Var n, b) =>
             match nth_error u n with
-            | Some l => match NoPropLevel.of_level l with
-                       | inl l => UnivExpr.npe (l, b)
-                       | inr _ =>
-                         (* CHECKME:SPROP: should we return [SProp] in some cases? *)
-                         if b then UnivExpr.type1 else UnivExpr.lProp
-                       end
+            | Some l => UnivExpr.npe (NoPropLevel.of_level l,b)
             | None => UnivExpr.npe (NoPropLevel.lSet, b)
             end
           end.
 
 Instance subst_instance_univ : UnivSubst Universe.t :=
-  fun u s => Universe.map (subst_instance_level_expr u) s.
+  fun u e => match e with
+          | Universe.lProp | Universe.lSProp => e
+          | Universe.lnpe l =>
+            Universe.lnpe (Universe.map (subst_instance_level_expr u) l)
+          end.
 
 Instance subst_instance_instance : UnivSubst Instance.t :=
   fun u u' => List.map (subst_instance_level u) u'.
@@ -1668,8 +1698,14 @@ Section Closedu.
   Definition closedu_level_expr (s : UnivExpr.t) :=
     closedu_level (UnivExpr.get_level s).
 
-  Definition closedu_universe (u : Universe.t) :=
+  Definition closedu_universe_levels (u : Universe.t0) :=
     UnivExprSet.for_all closedu_level_expr u.
+
+  Definition closedu_universe (u : Universe.t) :=
+    match u with
+    | Universe.lSProp | Universe.lProp => true
+    | Universe.lnpe l => closedu_universe_levels l
+    end.
 
   Definition closedu_instance (u : Instance.t) :=
     forallb closedu_level u.
@@ -1686,13 +1722,18 @@ Section UniverseClosedSubst.
   Lemma closedu_subst_instance_level_expr u e
     : closedu_level_expr 0 e -> subst_instance_level_expr u e = e.
   Proof.
-    destruct e as [| |[[] b]]; cbnr. discriminate.
+    intros.
+    destruct e as [[t b]]. destruct t;cbnr. discriminate.
   Qed.
 
   Lemma closedu_subst_instance_univ u s
     : closedu_universe 0 s -> subst_instance_univ u s = s.
   Proof.
-    intro H. apply eq_univ'.
+    intro H.
+    destruct s;auto;cbn in *.
+    apply f_equal. apply eq_univ'.
+    destruct t as [ts H1].
+    unfold closedu_universe_levels in *;cbn in *.
     intro e; split; intro He.
     - apply Universe.map_spec in He. destruct He as [e' [He' X]].
       rewrite closedu_subst_instance_level_expr in X.
@@ -1711,6 +1752,7 @@ Section UniverseClosedSubst.
     apply closedu_subst_instance_level.
     eapply forallb_forall in H; eassumption.
   Qed.
+
 End UniverseClosedSubst.
 
 Hint Resolve closedu_subst_instance_level closedu_subst_instance_level_expr
@@ -1734,18 +1776,21 @@ Section SubstInstanceClosed.
   Lemma subst_instance_level_expr_closedu e :
     closedu_level_expr #|u| e -> closedu_level_expr 0 (subst_instance_level_expr u e).
   Proof.
-    destruct e as [| |[[] b]]; cbnr.
+    destruct e;cbnr.
+    destruct e as [l b]. destruct l;cbnr.
     case_eq (nth_error u n); cbnr. intros [] Hl X; cbnr.
-    now destruct b. apply nth_error_In in Hl.
+    apply nth_error_In in Hl.
     eapply forallb_forall in Hcl; tea.
-    (* discriminate. *)
-    (* Qed. *)
-    Admitted.
+    discriminate.
+  Qed.
 
   Lemma subst_instance_univ_closedu s
     : closedu_universe #|u| s -> closedu_universe 0 (subst_instance_univ u s).
   Proof.
-    intro H. apply UnivExprSet.for_all_spec; proper.
+    intro H.
+    destruct s;cbnr.
+    destruct t as [l Hl].
+    apply UnivExprSet.for_all_spec; proper.
     intros e He. eapply Universe.map_spec in He.
     destruct He as [e' [He' X]]; subst.
     apply subst_instance_level_expr_closedu.
@@ -1768,8 +1813,6 @@ Hint Resolve subst_instance_level_closedu subst_instance_level_expr_closedu
 
 Definition string_of_level (l : Level.t) : string :=
   match l with
-  | Level.lSProp => "SProp"
-  | Level.lProp => "Prop"
   | Level.lSet => "Set"
   | Level.Level s => s
   | Level.Var n => "Var" ^ string_of_nat n
@@ -1777,17 +1820,18 @@ Definition string_of_level (l : Level.t) : string :=
 
 Definition string_of_level_expr (e : UnivExpr.t) : string :=
   match e with
-  | UnivExpr.lSProp => "SProp"
-  | UnivExpr.lProp => "Prop"
   | UnivExpr.npe (l, b) => string_of_level l ^ (if b then "+1" else "")
   end.
 
 Definition string_of_sort (u : Universe.t) :=
-  string_of_list string_of_level_expr (UnivExprSet.elements u).
+  match u with
+  | Universe.lSProp => "SProp"
+  | Universe.lProp => "Prop"
+  | Universe.lnpe l => string_of_list string_of_level_expr (UnivExprSet.elements l)
+  end.
 
 Definition string_of_universe_instance u :=
   string_of_list string_of_level u.
-
 
 Inductive universes_entry :=
 | Monomorphic_entry (ctx : ContextSet.t)
@@ -1829,6 +1873,14 @@ Definition print_constraint_set t :=
              " /\ " (ConstraintSet.elements t).
 
 
+Lemma val_universe_sup_not_prop vv v u :
+  Universe.is_prop v = false -> Universe.is_sprop v = false ->
+  0 <= val vv (Universe.universe_sup u v).
+Proof.
+  intros Hp Hsp.
+  destruct u,v;cbn;try discriminate;try lia; try apply val_zero_exprs.
+Qed.
+
 Lemma leq_universe_product_mon {cf: checker_flags} ϕ u u' v v' :
   leq_universe ϕ u u' ->
   leq_universe ϕ v v' ->
@@ -1838,19 +1890,32 @@ Proof.
   intros H1 H2 vv Hv. specialize (H1 _ Hv). specialize (H2 _ Hv).
   cbn in *. unfold Universe.sort_of_product.
   destruct (Universe.is_prop v) eqn:e, (Universe.is_prop v') eqn:f;
-    rewrite ?val_sup.
+    destruct (Universe.is_sprop v) eqn:e1, (Universe.is_sprop v') eqn:f1;
+    rewrite ?val_sup;cbn;auto.
+  - destruct v;discriminate.
   - apply is_prop_val with (v:=vv) in e.
-    apply is_prop_val with (v:=vv) in f.
-    now rewrite e, f.
-  - apply is_prop_val with (v:=vv) in e.
-    apply is_prop_val_false with (v:=vv) in f.
-    lled; lia.
-  - apply is_prop_val_false with (v:=vv) in e.
-    apply is_prop_val with (v:=vv) in f.
-    lled; lia.
-  - apply is_prop_val_false with (v:=vv) in e.
-    apply is_prop_val_false with (v:=vv) in f.
-    lled; lia.
+    specialize (is_prop_and_is_sprop_val_false _ f f1 vv) as HH.
+    specialize (val_universe_sup_not_prop vv _ u' f f1) as HH1.
+    lled; try lia.
+  - destruct v';discriminate.
+  - apply is_prop_val with (v:=vv) in f.
+    specialize (is_prop_and_is_sprop_val_false _ e e1 vv) as HH.
+    specialize (val_universe_sup_not_prop vv _ u' e e1) as HH1.
+    lled; try lia.
+  - apply is_sprop_val with (v:=vv) in e1.
+    specialize (is_prop_and_is_sprop_val_false _ f f1 vv) as HH.
+    specialize (val_universe_sup_not_prop vv _ u' f f1) as HH1.
+    lled; try lia.
+  -apply is_sprop_val with (v:=vv) in f1.
+    specialize (is_prop_and_is_sprop_val_false _ e e1 vv) as HH.
+    specialize (val_universe_sup_not_prop vv _ u' e e1) as HH1.
+    lled; try lia.
+  - specialize (is_prop_and_is_sprop_val_false _ e e1 vv) as HH.
+    specialize (val_universe_sup_not_prop vv _ u' e e1) as HH1.
+    specialize (is_prop_and_is_sprop_val_false _ f f1 vv) as HH'.
+    specialize (val_universe_sup_not_prop vv _ u' f f1) as HH1'.
+    repeat rewrite val_universe_sup.
+    lled; try lia.
 Qed.
 
 Lemma impredicative_product {cf:checker_flags} {ϕ l u} :
@@ -1860,7 +1925,6 @@ Proof.
   unfold Universe.sort_of_product.
   intros ->. reflexivity.
 Qed.
-
 
 Section UniverseLemmas.
   Context {cf:checker_flags}.
@@ -1874,11 +1938,20 @@ Section UniverseLemmas.
     intro; rewrite !UnivExprSet.union_spec. intuition.
   Qed.
 
+  Lemma universe_sup_idem s : Universe.universe_sup s s = s.
+  Proof.
+    destruct s;cbn;auto.
+    apply f_equal.
+    apply eq_univ'; cbn.
+    intro; rewrite !UnivExprSet.union_spec. intuition.
+  Qed.
+
   Lemma sort_of_product_idem s
     : Universe.sort_of_product s s = s.
   Proof.
-    unfold Universe.sort_of_product. destruct (Universe.is_prop s); trea.
-    apply sup_idem.
+    unfold Universe.sort_of_product.
+    destruct (Universe.is_prop s), (Universe.is_sprop s); trea;cbn.
+    apply universe_sup_idem.
   Qed.
 
   Lemma sup_assoc s1 s2 s3 :
@@ -1887,22 +1960,20 @@ Section UniverseLemmas.
     apply eq_univ'; cbn. symmetry; apply UnivExprSetProp.union_assoc.
   Qed.
 
-  Instance sup_eq_universe φ :
-    Proper (eq_universe φ ==> eq_universe φ ==> eq_universe φ) Universe.sup.
+  Instance universe_sup_eq_universe φ :
+    Proper (eq_universe φ ==> eq_universe φ ==> eq_universe φ) Universe.universe_sup.
   Proof.
     intros s1 s1' H1 s2 s2' H2.
     unfold_eq_universe. specialize (H1 v Hv). specialize (H2 v Hv).
-    rewrite !val_sup; lia.
+    rewrite !val_universe_sup. lia.
   Qed.
 
   Lemma sort_of_product_twice u s :
     Universe.sort_of_product u (Universe.sort_of_product u s)
     = Universe.sort_of_product u s.
   Proof.
-    apply eq_univ'.
-    unfold Universe.sort_of_product. case_eq (Universe.is_prop s).
-    - intros ->. reflexivity.
-    - intro e. rewrite is_prop_sup, e, andb_false_r.
+    destruct u,s;auto.
+    unfold Universe.sort_of_product;cbn.
     now rewrite sup_assoc, sup_idem.
   Qed.
 End UniverseLemmas.
@@ -1920,39 +1991,73 @@ Section no_prop_leq_type.
     leq_universe ϕ (Universe.super l) (Universe.super l').
   Proof.
     unfold leq_universe. destruct check_univs; [|trivial].
-    intros H v Hv. specialize (H v Hv). cbn in *.
+    intros H v Hv. specialize (H v Hv). simpl in *.
     destruct l, l'; lled; cbn -[Z.add] in *; destruct H; lia.
   Qed.
 
-  Lemma leq_universe_prop u1 u2 :
+  Hint Resolve lle_le val_is_prop_or_sprop : univ_lemmas.
+
+  Lemma leq_universe_prop_sprop u1 u2 :
     check_univs ->
     consistent ϕ ->
     leq_universe ϕ u1 u2 ->
-    Universe.is_prop u2 -> Universe.is_prop u1.
+    Universe.is_prop u2 -> Universe.is_prop u1 \/ Universe.is_sprop u1.
   Proof.
     intros Hcf [v Hv] H1 H2.
-    eapply is_prop_val in H2. (* eapply (val_is_prop _ v). *)
-  (*   unfold leq_universe in *. rewrite Hcf in H1. *)
-  (*   specialize (H1 _ Hv). rewrite H2 in H1. *)
-  (*   cbn in *. lled; lia. *)
-    (* Qed. *)
-    Admitted.
+    apply is_prop_val with (v:=v) in H2.
+    unfold leq_universe in *. rewrite Hcf in H1.
+    specialize (H1 _ Hv). rewrite H2 in H1. cbn in *.
+    eauto with univ_lemmas.
+  Qed.
+
+  Lemma leq_universe_sprop_prop u1 u2 :
+    check_univs ->
+    consistent ϕ ->
+    leq_universe ϕ u1 u2 ->
+    Universe.is_sprop u2 -> Universe.is_prop u1 \/ Universe.is_sprop u1.
+  Proof.
+    intros Hcf [v Hv] H1 H2.
+    apply is_sprop_val with (v:=v) in H2.
+    unfold leq_universe in *. rewrite Hcf in H1.
+    specialize (H1 _ Hv). rewrite H2 in H1. cbn in *.
+    eauto with univ_lemmas.
+  Qed.
 
   Lemma leq_universe_prop_no_prop_sub_type u1 u2 :
     check_univs ->
     prop_sub_type = false ->
     consistent ϕ ->
     leq_universe ϕ u1 u2 ->
-    Universe.is_prop u1 -> Universe.is_prop u2.
+    Universe.is_prop u1 -> Universe.is_prop u2 \/ Universe.is_sprop u2.
   Proof.
     intros Hcf npst [v Hv] H1 H2.
-    eapply is_prop_val in H2.
-    (* eapply (val_is_prop _ v). *)
-  (*   unfold leq_universe in *. rewrite Hcf in H1. *)
-  (*   specialize (H1 _ Hv). rewrite H2 in H1. *)
-  (*   cbn in *. lled; lia. *)
-    (* Qed. *)
-    Admitted.
+    apply is_prop_val with (v:=v) in H2.
+    unfold leq_universe in *. rewrite Hcf in H1.
+    apply val_is_prop_or_sprop with (v:=v).
+    specialize (H1 _ Hv). rewrite H2 in H1.
+    cbn in *. lled; lia.
+  Qed.
+
+  Lemma leq_universe_sprop_no_prop_sub_type u1 u2 :
+    check_univs ->
+    prop_sub_type = false ->
+    consistent ϕ ->
+    leq_universe ϕ u1 u2 ->
+    Universe.is_sprop u1 -> Universe.is_prop u2 \/ Universe.is_sprop u2.
+  Proof.
+    intros Hcf npst [v Hv] H1 H2.
+    apply is_sprop_val with (v:=v) in H2.
+    unfold leq_universe in *. rewrite Hcf in H1.
+    apply val_is_prop_or_sprop with (v:=v).
+    specialize (H1 _ Hv). rewrite H2 in H1.
+    cbn in *. lled; lia.
+  Qed.
+
+
+  Hint Resolve leq_universe_sprop_prop
+       leq_universe_prop_sprop
+       leq_universe_prop_no_prop_sub_type
+       leq_universe_sprop_no_prop_sub_type : univ_lemmas.
 
   Lemma leq_prop_prop {l l'} :
     Universe.is_prop l -> Universe.is_prop l' ->
@@ -1963,16 +2068,14 @@ Section no_prop_leq_type.
     rewrite H1, H2. lled; lia.
   Qed.
 
-  Lemma leq_prop_is_prop {x s} :
+  Lemma leq_prop_is_prop_sprop {x s} :
     check_univs ->
     prop_sub_type = false ->
     consistent ϕ ->
     leq_universe ϕ x s ->
-    (Universe.is_prop s <-> Universe.is_prop x).
+    (Universe.is_prop s \/ Universe.is_sprop s <-> Universe.is_prop x \/ Universe.is_sprop x).
   Proof.
-    intros H H0 H1 H2; split.
-    now apply leq_universe_prop.
-    now apply leq_universe_prop_no_prop_sub_type.
+    intros H H0 H1 H2; split;intros Hor; destruct Hor; eauto with univ_lemmas.
   Qed.
 
   Lemma is_prop_gt l l' :
